/ dhall-lang Public

# How to translate recursive code to Dhall

This page has moved to `docs.dhall-lang.org` - How to translate recursive code to Dhall

This copy of the page will no longer be kept up-to-date

The Dhall configuration language only provides built-in support for one recursive data type: `List`s. However, the language does not provide native support for user-defined recursive types, recursive values, or recursive functions.

Despite that limitation, you can still transform recursive code into non-recursive Dhall code. This guide will explain how by example, walking through examples of progressively increasing difficulty.

## Recursive record

Consider the following recursive Haskell code:

```-- Example0.hs

data Person = MakePerson
{ name     :: String
, children :: [Person]
}

example :: Person
example =
MakePerson
{ name     = "John"
, children =
[ MakePerson { name = "Mary", children = [] }
, MakePerson { name = "Jane", children = [] }
]
}

everybody :: Person -> [String]
everybody p = name p : concatMap everybody (children p)

result :: [String]
result = everybody example```

... which evaluates to:

```\$ ghci Example0.hs
*Main> result
["John","Mary","Jane"]```

The equivalent Dhall code would be:

```-- example0.dhall

let Person
: Type
=   ∀(Person : Type)
→ ∀(MakePerson : { children : List Person, name : Text } → Person)
→ Person

let example
: Person
=   λ(Person : Type)
→ λ(MakePerson : { children : List Person, name : Text } → Person)
→ MakePerson
{ children =
[ MakePerson { children = [] : List Person, name = "Mary" }
, MakePerson { children = [] : List Person, name = "Jane" }
]
, name =
"John"
}

let everybody
: Person → List Text
= let concat = http://prelude.dhall-lang.org/List/concat

in    λ(x : Person)
→ x
(List Text)
(   λ(p : { children : List (List Text), name : Text })
→ [ p.name ] # concat Text p.children
)

let result : List Text = everybody example

in  result```

... which evaluates to the same result:

```\$ dhall <<< './example0.dhall'
List Text

[ "John", "Mary", "Jane" ]```

Carefully note that there is more than one bound variable named `Person` in the above example. We can disambiguate them by prefixing some of them with an underscore (i.e. `_Person`):

```let Person
: Type
=   ∀(_Person : Type)
→ ∀(MakePerson : { children : List _Person, name : Text } → _Person)
→ _Person

let example
: Person
=   λ(_Person : Type)
→ λ(MakePerson : { children : List _Person, name : Text } → _Person)
→ MakePerson
{ children =
[ MakePerson { children = [] : List _Person, name = "Mary" }
, MakePerson { children = [] : List _Person, name = "Jane" }
]
, name =
"John"
}

let everybody
: Person → List Text
= let concat = http://prelude.dhall-lang.org/List/concat

in    λ(x : Person)
→ x
(List Text)
(   λ(p : { children : List (List Text), name : Text })
→ [ p.name ] # concat Text p.children
)

let result : List Text = everybody example

in  result```

The way that this works is that a recursive function like `everybody` is performing substitution. In this specific case, `everybody` is:

• replacing each occurrence of the type `Person` with the type `List Text`

• replacing each occurrence of the `MakePerson` function with the following anonymous function:

```   λ(p : { children : List (List Text), name : Text })
→ [ p.name ] # concat Text p.children```

... which means that our previous example could also have been written like this:

```let concat = http://prelude.dhall-lang.org/List/concat

let Person : Type = List Text

let MakePerson
: { children : List Person, name : Text } → Person
=   λ(p : { children : List Person, name : Text })
→ [ p.name ] # concat Text p.children

let result =
MakePerson
{ children =
[ MakePerson { children = [] : List Person, name = "Mary" }
, MakePerson { children = [] : List Person, name = "Jane" }
]
, name =
"John"
}

in  result```

## Recursive sum type

Sum types work in the same way, except that instead of one constructor (i.e. `MakePerson`) we now have two constructors: `Succ` and `Nat`. For example, this Haskell code:

```-- Example1.hs

import Numeric.Natural (Natural)

data Nat = Zero | Succ Nat

example :: Nat
example = Succ (Succ (Succ Zero))

toNatural :: Nat -> Natural
toNatural  Zero    = 0
toNatural (Succ n) = 1 + toNatural n

result :: Natural
result = toNatural example```

... which produces this `result`:

```\$ ghci Example1.hs
*Main> result
3```

... corresponds to this Dhall code:

```-- example1.dhall

let Nat : Type = ∀(Nat : Type) → ∀(Zero : Nat) → ∀(Succ : Nat → Nat) → Nat

let example
: Nat
=   λ(Nat : Type)
→ λ(Zero : Nat)
→ λ(Succ : Nat → Nat)
→ Succ (Succ (Succ Zero))

let toNatural
: Nat → Natural
= λ(x : Nat) → x Natural 0 (λ(n : Natural) → 1 + n)

let result : Natural = toNatural example

in  result```

... which produces the same `result`:

```\$ dhall <<< './example1.dhall'
Natural

3```

Like before, our recursive `toNatural` function is performing substitution by:

• replacing every occurrence of `Nat` with `Natural`
• replacing every occurrence of `Zero` with `0`
• replacing every occurrence of `Succ` with an anonymous funciton

... which means that we could have equivalently written:

```let Nat = Natural

let Zero : Nat = 0

let Succ : Nat → Nat = λ(n : Nat) → 1 + n

let result : Nat = Succ (Succ (Succ Zero))

in  result```

## Mutually recursive types

The above pattern generalizes to mutually recursive types, too. For example, this Haskell code:

```-- Example2.hs

import Numeric.Natural

data Even = Zero | SuccEven Odd

data Odd = SuccOdd Even

example :: Odd
example = SuccOdd (SuccEven (SuccOdd Zero))

oddToNatural :: Odd -> Natural
oddToNatural (SuccOdd e) = 1 + evenToNatural e

evenToNatural :: Even -> Natural
evenToNatural  Zero        = 0
evenToNatural (SuccEven o) = 1 + oddToNatural o

result :: Natural
result = oddToNatural example```

... which produces this `result`:

```\$ ghci Example2.hs
*Main> result
3```

... corresponds to this Dhall code:

```let Odd
: Type
=   ∀(Even : Type)
→ ∀(Odd : Type)
→ ∀(Zero : Even)
→ ∀(SuccEven : Odd → Even)
→ ∀(SuccOdd : Even → Odd)
→ Odd

let example
: Odd
=   λ(Even : Type)
→ λ(Odd : Type)
→ λ(Zero : Even)
→ λ(SuccEven : Odd → Even)
→ λ(SuccOdd : Even → Odd)
→ SuccOdd (SuccEven (SuccOdd Zero))

let oddToNatural
: Odd → Natural
=   λ(o : Odd)
→ o Natural Natural 0 (λ(n : Natural) → 1 + n) (λ(n : Natural) → 1 + n)

let result = oddToNatural example

in  result```

... which produces the same `result`:

```\$ dhall <<< './example2.dhall'
Natural

3```

The trick here is that the Dhall's `Odd` type combines both of the Haskell `Even` and `Odd` types. Similarly, Dhall's `oddToNatural` function combines both of the Haskell `evenToNatural` and `oddToNatural` functions. You can define a separate `Even` and `evenToNatural` in Dhall, too, but they would not reuse any of the logic from `Odd` or `oddToNatural`.

Like before, our recursive `oddToNatural` function is performing substitution by:

• replacing every occurrence of `Even` with `Natural`
• replacing every occurrence of `Odd` with `Natural`
• replacing every occurrence of `Zero` with `0`
• replacing every occurrence of `SuccEven` with an anonymous function
• replacing every occurrence of `SuccOdd` with an anonymous function

... which means that we could have equivalently written:

```let Odd : Type = Natural

let Even : Type = Natural

let Zero : Even = 0

let SuccEven : Odd → Even = λ(n : Odd) → 1 + n

let SuccOdd : Even → Odd = λ(n : Even) → 1 + n

let result = SuccOdd (SuccEven (SuccOdd Zero))

in  result```

## JSON

You can see a real example of this pattern in the Prelude's support for `JSON`

## Conclusion

The general algorithm for translating recursive code to non-recursive code is known as Boehm Berarducci encoding and based off of this paper:

This guide doesn't explain the full algorithm due to the amount of detail involved, but if you are interested you can read the above paper.

Also, if the above examples were not sufficient, feel free to open an issue to request another example to add to this guide.